proof/correctness/IndcpaDerand.ec
@@ -1,0 +1,601 @@
+require import List Int IntExtra IntDiv CoreMap.
+from Jasmin require import JModel.
+
+require import Array4 Array5 Array24 Array25 Array32 Array33 Array34 Array64
+               Array128 Array168 Array256 Array768.
+require import WArray20 WArray32 WArray33 WArray34 WArray40 WArray64
+               WArray128 WArray168 WArray192 WArray200 WArray256 WArray512
+               WArray1536.
+
+require import Indcpa.
+
+print M.
+(* WE DEFINE ALTERNATIVE VERSIONS OF THE EXTRACTED CODE TO
+   MODULARIZE RANDOMNESS SAMPLINGS *)
+
+op scoins : W8.t Array32.t distr.
+
+module Mderand = {
+  include M [-indcpa_keypair_jazz, indcpa_enc_jazz, indcpa_dec_jazz, poly_compress, poly_decompress, polyvec_compress, polyvec_decompress]
+
+ proc poly_compress_round(a : W16.t Array256.t) : W16.t Array256.t = {
+    var aux : int;
+    var i : int;
+    var t : W16.t;
+    var d0 : W32.t;
+    var d1 : W32.t;
+    var r : W16.t Array256.t;
+    
+    a <@ M.poly_csubq(a);
+
+    r <- witness;
+    i <- 0;
+    while (i < 128){
+      t <- a.[2 * i];
+      d0 <- zeroextu32 t;
+      d0 <- d0 `<<` (of_int 4)%W8;
+      d0 <- d0 + (of_int 1665)%W32;
+      d0 <- d0 * (of_int 80635)%W32;
+      d0 <- d0 `>>` (of_int 28)%W8;
+      d0 <- d0 `&` (of_int 15)%W32;
+      t <- a.[2 * i + 1];
+      d1 <- zeroextu32 t;
+      d1 <- d1 `<<` (of_int 4)%W8;
+      d1 <- d1 + (of_int 1665)%W32;
+      d1 <- d1 * (of_int 80635)%W32;
+      d1 <- d1 `>>` (of_int 28)%W8;
+      d1 <- d1 `&` (of_int 15)%W32;
+      r.[2*i] <- truncateu16 d0;
+      r.[2*i+1]<- truncateu16 d1;
+      i <- i + 1;
+    }
+    
+    return r;
+  }
+  
+ proc poly_compress_store(rp : W64.t, r : W16.t Array256.t) : unit = {
+    var aux : int;
+    var i : int;
+    var d0 : W16.t;
+    var d1 : W16.t;
+    i <- 0;
+    while (i < 128){
+      d0 <- r.[2*i];
+      d1 <- r.[2*i+1];
+      d1 <- d1 `<<` (of_int 4)%W8;
+      d0 <- d0 `|` d1;
+      Glob.mem <- storeW8 Glob.mem (to_uint (rp + (of_int i)%W64)) (truncateu8 d0);
+      i <- i + 1;
+    }
+    
+    return tt;
+  }
+  
+  proc poly_decompress_load(ap : W64.t) : W16.t Array256.t = {
+    var aux : int;
+    var rp : W16.t Array256.t;
+    var i : int;
+    var t : W8.t;
+    var d0 : W16.t;
+    var d1 : W16.t;
+    
+    rp <- witness;
+    i <- 0;
+    while (i < 128){
+      t <- loadW8 Glob.mem (to_uint (ap + (of_int i)%W64));
+      d0 <- zeroextu16 t;
+      d1 <- zeroextu16 t;
+      d0 <- d0 `&` (of_int 15)%W16;
+      d1 <- d1 `>>` (of_int 4)%W8;
+      rp.[2 * i] <- d0;
+      rp.[2 * i + 1] <- d1;
+      i <- i + 1;
+    }
+    
+    return rp;
+  }
+
+  proc poly_decompress_restore(r : W16.t Array256.t) : W16.t Array256.t = {
+    var aux : int;
+    var rp : W16.t Array256.t;
+    var i : int;
+    var d0 : W16.t;
+    var d1 : W16.t;
+    
+    rp <- witness;
+    i <- 0;
+    while (i < 128){
+      d0 <- r.[2*i];
+      d1 <- r.[2*i+1];
+      d0 <- d0 * (of_int 3329)%W16;
+      d1 <- d1 * (of_int 3329)%W16;
+      d0 <- d0 + (of_int 8)%W16;
+      d1 <- d1 + (of_int 8)%W16;
+      d0 <- d0 `>>` (of_int 4)%W8;
+      d1 <- d1 `>>` (of_int 4)%W8;
+      rp.[2 * i] <- d0;
+      rp.[2 * i + 1] <- d1;
+      i <- i + 1;
+    }
+    
+    return rp;
+  }
+
+
+
+ proc polyvec_compress_round( a : W16.t Array768.t) : W16.t Array768.t = {
+    var i : W64.t;
+    var aa : W16.t Array768.t;
+    var r : W16.t Array768.t;
+    var k : int;
+    var t : W64.t Array4.t;
+    
+    t <- witness;
+    r <- witness;
+    i <- W64.zero;
+    aa <@ M.polyvec_csubq(a);
+    while (i \ult (of_int 768)%W64){
+      k <- 0;
+      while (k < 4){
+        t.[k] <- zeroextu64 aa.[to_uint i];
+        i <- i + W64.one;
+        t.[k] <- t.[k] `<<` (of_int 10)%W8;
+        t.[k] <- t.[k] + (of_int 1665)%W64;
+        t.[k] <- t.[k] * (of_int 1290167)%W64;
+        t.[k] <- t.[k] `>>` (of_int 32)%W8;
+        t.[k] <- t.[k] `&` (of_int 1023)%W64;
+        k <- k + 1;
+      }
+      r.[to_uint i-4] <- truncateu16 t.[k-4];
+      r.[to_uint i-3] <- truncateu16 t.[k-3];
+      r.[to_uint i-2] <- truncateu16 t.[k-2];
+      r.[to_uint i-1] <- truncateu16 t.[k-1];
+    }
+    
+    return r;
+  }
+
+ proc polyvec_compress_store(rp : W64.t, r : W16.t Array768.t) : unit = {
+    var aux : int;
+    var i : W64.t;
+    var j : W64.t;
+    var k : int;
+    var t : W16.t Array4.t;
+    var c : W16.t;
+    var b : W16.t;
+    
+    t <- witness;
+    i <- W64.zero;
+    j <- W64.zero;
+    while (i \ult (of_int 768)%W64){
+      k <- 0;
+      while (k < 4){
+        t.[k] <- r.[to_uint i];
+        i <- i + W64.one;
+        k <- k + 1;
+      }
+      c <- t.[0];
+      c <- c `&` (of_int 255)%W16;
+      Glob.mem <- storeW8 Glob.mem (to_uint (rp + j)) (truncateu8 c);
+      j <- j + W64.one;
+      b <- t.[0];
+      b <- b `>>` (of_int 8)%W8;
+      c <- t.[1];
+      c <- c `<<` (of_int 2)%W8;
+      c <- c `|` b;
+      Glob.mem <- storeW8 Glob.mem (to_uint (rp + j)) (truncateu8 c);
+      j <- j + W64.one;
+      b <- t.[1];
+      b <- b `>>` (of_int 6)%W8;
+      c <- t.[2];
+      c <- c `<<` (of_int 4)%W8;
+      c <- c `|` b;
+      Glob.mem <- storeW8 Glob.mem (to_uint (rp + j)) (truncateu8 c);
+      j <- j + W64.one;
+      b <- t.[2];
+      b <- b `>>` (of_int 4)%W8;
+      c <- t.[3];
+      c <- c `<<` (of_int 6)%W8;
+      c <- c `|` b;
+      Glob.mem <- storeW8 Glob.mem (to_uint (rp + j)) (truncateu8 c);
+      j <- j + W64.one;
+      t.[3] <- t.[3] `>>` (of_int 2)%W8;
+      Glob.mem <- storeW8 Glob.mem (to_uint (rp + j)) (truncateu8 t.[3]);
+      j <- j + W64.one;
+    }
+    
+    return tt;
+  }
+  
+  proc polyvec_decompress_load(ap : W64.t) : W32.t Array768.t = {
+    var aux : int;
+    var r : W32.t Array768.t;
+    var i : W64.t;
+    var j : W64.t;
+    var k : int;
+    var t : W32.t Array5.t;
+    var d : W32.t;
+    
+    r <- witness;
+    t <- witness;
+    i <- W64.zero;
+    j <- W64.zero;
+    while (i \ult (of_int 768)%W64){
+      k <- 0;
+      while (k < 5){
+        t.[k] <- zeroextu32 (loadW8 Glob.mem (to_uint (ap + j)));
+        j <- j + W64.one;
+        k <- k + 1;
+      }
+      d <- t.[1];
+      t.[1] <- t.[1] `>>` (of_int 2)%W8;
+      d <- d `&` (of_int 3)%W32;
+      d <- d `<<` (of_int 8)%W8;
+      t.[0] <- t.[0] `|` d;
+      d <- t.[2];
+      t.[2] <- t.[2] `>>` (of_int 4)%W8;
+      d <- d `&` (of_int 15)%W32;
+      d <- d `<<` (of_int 6)%W8;
+      t.[1] <- t.[1] `|` d;
+      d <- t.[3];
+      t.[3] <- t.[3] `>>` (of_int 6)%W8;
+      d <- d `&` (of_int 63)%W32;
+      d <- d `<<` (of_int 4)%W8;
+      t.[2] <- t.[2] `|` d;
+      d <- t.[4];
+      d <- d `<<` (of_int 2)%W8;
+      t.[3] <- t.[3] `|` d;
+      k <- 0;
+      while (k < 4){
+        r.[to_uint i] <-  t.[k];
+        i <- i + W64.one;
+        k <- k + 1;
+      }
+    }
+    
+    return r;
+  }
+
+  proc polyvec_decompress_restore(rp : W32.t Array768.t) : W16.t Array768.t = {
+    var aux : int;
+    var r : W16.t Array768.t;
+    var i : W64.t;
+    var j : W64.t;
+    var k : int;
+    var t : W32.t Array5.t;
+    var d : W32.t;
+    
+    r <- witness;
+    t <- witness;
+    i <- W64.zero;
+    j <- W64.zero;
+    while (i \ult (of_int 768)%W64){
+      k <- 0;
+      while (k < 5){
+        t.[k] <- rp.[to_uint i];
+        j <- j + W64.one;
+        k <- k + 1;
+      }
+      k <- 0;
+      while (k < 4){
+        t.[k] <- t.[k] * (of_int 3329)%W32;
+        t.[k] <- t.[k] + (of_int 512)%W32;
+        t.[k] <- t.[k] `>>` (of_int 10)%W8;
+        r.[to_uint i] <- truncateu16 t.[k];
+        i <- i + W64.one;
+        k <- k + 1;
+      }
+    }
+    
+    return r;
+  }
+
+  proc indcpa_keypair_expandseed(randomnessp:W64.t) : 
+    W8.t Array32.t *  W16.t Array768.t * W16.t Array768.t = {
+    var i:W64.t;
+    var c:W8.t;
+    var inbuf:W8.t Array32.t;
+    var buf:W8.t Array64.t;
+    var j:W64.t;
+    var publicseed:W8.t Array32.t;
+    var noiseseed:W8.t Array32.t;
+    var nonce:W8.t;
+    var poly0:W16.t Array256.t;
+    var poly1:W16.t Array256.t;
+    var poly2:W16.t Array256.t;
+    var skpv:W16.t Array768.t;
+    var e:W16.t Array768.t;
+
+    inbuf <- witness;
+    noiseseed <- witness;
+    publicseed <- witness;
+
+    i <- (W64.of_int 0);
+    
+    while ((i \ult (W64.of_int 32))) {
+      c <- (loadW8 Glob.mem (W64.to_uint (randomnessp + i)));
+      inbuf.[(W64.to_uint i)] <- c;
+      i <- (i + (W64.of_int 1));
+    }
+    buf <@ sha3512_32 (inbuf);
+    i <- (W64.of_int 0);
+    j <- (W64.of_int 32);
+    
+    while ((i \ult (W64.of_int 32))) {
+      c <- buf.[(W64.to_uint i)];
+      publicseed.[(W64.to_uint i)] <- c;
+      c <- buf.[(W64.to_uint j)];
+      noiseseed.[(W64.to_uint i)] <- c;
+      i <- (i + (W64.of_int 1));
+      j <- (j + (W64.of_int 1));
+    }
+    nonce <- (W8.of_int 0);
+    poly0 <@ poly_getnoise (noiseseed, nonce);
+    nonce <- (nonce + (W8.of_int 1));
+    poly1 <@ poly_getnoise (noiseseed, nonce);
+    nonce <- (nonce + (W8.of_int 1));
+    poly2 <@ poly_getnoise (noiseseed, nonce);
+    skpv <@ polyvec_frompolys (poly0, poly1, poly2);
+    nonce <- (nonce + (W8.of_int 1));
+    poly0 <@ poly_getnoise (noiseseed, nonce);
+    nonce <- (nonce + (W8.of_int 1));
+    poly1 <@ poly_getnoise (noiseseed, nonce);
+    nonce <- (nonce + (W8.of_int 1));
+    poly2 <@ poly_getnoise (noiseseed, nonce);
+    e <@ polyvec_frompolys (poly0, poly1, poly2);
+    return (publicseed,e,skpv);
+  }
+
+  proc indcpa_keypair_compute(publicseed : W8.t Array32.t, e skpv : W16.t Array768.t) : 
+      W16.t Array768.t *  W16.t Array768.t = {
+    var poly0:W16.t Array256.t;
+    var poly1:W16.t Array256.t;
+    var poly2:W16.t Array256.t;
+    var pkpv:W16.t Array768.t;
+    var zero:W64.t;
+    var a0:W16.t Array768.t;
+    var a1:W16.t Array768.t;
+    var a2:W16.t Array768.t;
+
+    zero <- (W64.of_int 0);
+    (a0, a1, a2) <@ gen_matrix (publicseed, zero);
+    skpv <@ polyvec_ntt (skpv);
+    e <@ polyvec_ntt (e);
+    poly0 <@ polyvec_pointwise_acc (a0, skpv);
+    poly0 <@ poly_frommont (poly0);
+    poly1 <@ polyvec_pointwise_acc (a1, skpv);
+    poly1 <@ poly_frommont (poly1);
+    poly2 <@ polyvec_pointwise_acc (a2, skpv);
+    poly2 <@ poly_frommont (poly2);
+    pkpv <@ polyvec_frompolys (poly0, poly1, poly2);
+    pkpv <@ polyvec_add (pkpv, e);
+    pkpv <@ polyvec_reduce (pkpv);
+    return (skpv, pkpv);
+
+  }
+
+  proc indcpa_keypair_jazz (pkp:W64.t, skp:W64.t, randomnessp:W64.t) : unit = {
+    var i:W64.t;
+    var c:W8.t;
+    var publicseed:W8.t Array32.t;
+    var a0:W16.t Array768.t;
+    var a1:W16.t Array768.t;
+    var a2:W16.t Array768.t;
+    var e:W16.t Array768.t;
+    var skpv:W16.t Array768.t;
+    var pkpv:W16.t Array768.t;
+
+    (publicseed, e, skpv) <@ indcpa_keypair_expandseed(randomnessp);
+    (skpv, pkpv) <@ indcpa_keypair_compute(publicseed, e, skpv);
+
+    polyvec_tobytes (skp, skpv);
+    polyvec_tobytes (pkp, pkpv);
+
+    i <- (W64.of_int 0);
+    pkp <- (pkp + (W64.of_int (3 * 384)));
+    
+    while ((i \ult (W64.of_int 32))) {
+      c <- publicseed.[(W64.to_uint i)];
+      Glob.mem <- storeW8 Glob.mem (W64.to_uint (pkp + (W64.of_int 0))) c;
+      pkp <- (pkp + (W64.of_int 1));
+      i <- (i + (W64.of_int 1));
+    }
+    return ();
+  }
+
+  proc kg(pkp:W64.t, skp:W64.t, randomnessp:W64.t) : unit = {
+    var coins, i;
+    coins <$ scoins;
+    i <- 0;  
+    while (i < 32) {
+      Glob.mem <- storeW8 Glob.mem (W64.to_uint (randomnessp + (W64.of_int i))) coins.[i];
+      i <- i + 1;
+    }
+    indcpa_keypair_jazz(pkp, skp, randomnessp);
+  }
+  
+  proc indcpa_enc_expand_seed(coinsp:W64.t) :
+    W16.t Array768.t * W16.t Array768.t * W16.t Array256.t  = {
+    var i:W64.t;
+    var c:W8.t;
+    var noiseseed:W8.t Array32.t;
+    var poly0:W16.t Array256.t;
+    var poly1:W16.t Array256.t;
+    var poly2:W16.t Array256.t;
+    var sp_0:W16.t Array768.t;
+    var ep:W16.t Array768.t;
+    var epp:W16.t Array256.t;
+    var nonce:W8.t;
+
+    noiseseed <- witness;
+
+    i <- (W64.of_int 0);
+
+    while ((i \ult (W64.of_int 32))) {
+      c <- (loadW8 Glob.mem (W64.to_uint (coinsp + i)));
+      noiseseed.[(W64.to_uint i)] <- c;
+      i <- (i + (W64.of_int 1));
+    }
+    nonce <- (W8.of_int 0);
+    poly0 <@ poly_getnoise (noiseseed, nonce);
+    nonce <- (W8.of_int 1);
+    poly1 <@ poly_getnoise (noiseseed, nonce);
+    nonce <- (W8.of_int 2);
+    poly2 <@ poly_getnoise (noiseseed, nonce);
+    sp_0 <@ polyvec_frompolys (poly0, poly1, poly2);
+    nonce <- (W8.of_int 3);
+    poly0 <@ poly_getnoise (noiseseed, nonce);
+    nonce <- (W8.of_int 4);
+    poly1 <@ poly_getnoise (noiseseed, nonce);
+    nonce <- (W8.of_int 5);
+    poly2 <@ poly_getnoise (noiseseed, nonce);
+    ep <@ polyvec_frompolys (poly0, poly1, poly2);
+    nonce <- (W8.of_int 6);
+    epp <@ poly_getnoise (noiseseed, nonce);
+    return (sp_0,ep,epp);
+  }
+
+  proc indcpa_enc_compute(msgp:W64.t,publicseed:W8.t Array32.t, pkpv:W16.t Array768.t, sp_0 ep:W16.t Array768.t, epp:W16.t Array256.t) : W16.t Array768.t * W16.t Array256.t = {
+    var k:W16.t Array256.t;
+    var one:W64.t;
+    var at0:W16.t Array768.t;
+    var at1:W16.t Array768.t;
+    var at2:W16.t Array768.t;
+    var bp:W16.t Array768.t;
+    var v:W16.t Array256.t;
+    var poly0:W16.t Array256.t;
+    var poly1:W16.t Array256.t;
+    var poly2:W16.t Array256.t;
+    var r1:W16.t Array768.t;
+    var r2:W16.t Array256.t;
+
+    
+    k <@ poly_frommsg (msgp);
+    one <- (W64.of_int 1);
+    (at0, at1, at2) <@ gen_matrix (publicseed, one);
+    sp_0 <@ polyvec_ntt (sp_0);
+    poly0 <@ polyvec_pointwise_acc (at0, sp_0);
+    poly1 <@ polyvec_pointwise_acc (at1, sp_0);
+    poly2 <@ polyvec_pointwise_acc (at2, sp_0);
+    bp <@ polyvec_frompolys (poly0, poly1, poly2);
+    v <@ polyvec_pointwise_acc (pkpv, sp_0);
+    bp <@ polyvec_invntt (bp);
+    v <@ poly_invntt (v);
+    bp <@ polyvec_add (bp, ep);
+    v <@ poly_add (v, epp);
+    v <@ poly_add (v, k);
+    bp <@ polyvec_reduce (bp);
+    v <@ poly_reduce (v);
+    r1 <@polyvec_compress_round (bp);
+    r2 <@ poly_compress_round (v);
+    return (r1,r2);
+  }
+
+  proc indcpa_enc_jazz (ctp:W64.t, msgp:W64.t, pkp:W64.t, coinsp:W64.t) : unit = {
+    
+    var i:W64.t;
+    var c:W8.t;
+    var publicseed:W8.t Array32.t;
+    var sp_0:W16.t Array768.t;
+    var ep:W16.t Array768.t;
+    var epp:W16.t Array256.t;
+    var pkpv:W16.t Array768.t;
+    var r1:W16.t Array768.t;
+    var r2:W16.t Array256.t;
+
+    publicseed <- witness;
+    pkpv <@ polyvec_frombytes (pkp);
+    i <- (W64.of_int 0);
+    pkp <- (pkp + (W64.of_int (3 * 384)));
+    
+    while ((i \ult (W64.of_int 32))) {
+      c <- (loadW8 Glob.mem (W64.to_uint (pkp + (W64.of_int 0))));
+      publicseed.[(W64.to_uint i)] <- c;
+      pkp <- (pkp + (W64.of_int 1));
+      i <- (i + (W64.of_int 1));
+    }
+    (sp_0,ep,epp) <@ indcpa_enc_expand_seed(coinsp);
+    (r1,r2) <@ indcpa_enc_compute(msgp,publicseed,pkpv,sp_0,ep,epp);
+    polyvec_compress_store(ctp,r1);
+    ctp <- (ctp + (W64.of_int (3 * 320)));
+    poly_compress_store(ctp,r2);
+    return ();
+  }
+  
+  proc enc(ctp:W64.t, msgp:W64.t, pkp:W64.t, coinsp:W64.t) : unit = {
+    var coins, i;
+    coins <$ scoins;
+    i <- 0;  
+    while (i < 32) {
+      Glob.mem <- storeW8 Glob.mem (W64.to_uint (coinsp + (W64.of_int i))) coins.[i];
+      i <- i + 1;
+    }
+    indcpa_enc_jazz(ctp, msgp, pkp, coinsp);
+  }
+
+  proc indcpa_dec_compute(msgp:W64.t, r1 : W32.t Array768.t, r2 : W16.t Array256.t,skpv:W16.t Array768.t) : unit = {
+    var bp:W16.t Array768.t;
+    var v:W16.t Array256.t;
+    var mp:W16.t Array256.t;
+
+    bp <@ polyvec_decompress_restore (r1);
+    v <@ poly_decompress_restore (r2);
+    bp <@ polyvec_ntt (bp);
+    mp <@ polyvec_pointwise_acc (skpv, bp);
+    mp <@ poly_invntt (mp);
+    mp <@ poly_sub (v, mp);
+    mp <@ poly_reduce (mp);
+    poly_tomsg (msgp, mp);
+    return ();
+  }
+
+  proc indcpa_dec_jazz (msgp:W64.t, ctp:W64.t, skp:W64.t) : unit = {
+    
+    var skpv:W16.t Array768.t;
+    var r1 : W32.t Array768.t;
+    var r2 : W16.t Array256.t;
+
+    skpv <@ polyvec_frombytes (skp);
+    r1 <@ polyvec_decompress_load(ctp);
+    ctp <- (ctp + (W64.of_int (3 * 320)));
+    r2 <@ poly_decompress_load(ctp);
+
+    indcpa_dec_compute(msgp,r1,r2,skpv);
+    return ();
+  }
+
+}.
+
+equiv keypair_same :  M.indcpa_keypair_jazz ~ Mderand.indcpa_keypair_jazz :
+  ={arg,Glob.mem} ==> ={res,Glob.mem}.
+proc.
+inline Mderand.indcpa_keypair_expandseed Mderand.indcpa_keypair_compute. 
+by swap {1} [20..21] 14; sim.
+qed.
+
+equiv enc_same : M.indcpa_enc_jazz ~ Mderand.indcpa_enc_jazz :
+  ={arg,Glob.mem} ==> ={res,Glob.mem}.
+proc.
+inline Mderand.indcpa_enc_expand_seed Mderand.indcpa_enc_compute.
+swap {1} 9 -8.
+swap {1} 18 -16.
+swap {2} [6..9] -3.
+swap {1} [22..24] 16. 
+seq 53 48 : (={Glob.mem,bp,v,ctp}).
+sim; auto => />; call (_: ={Glob.mem}).
+by sim.
+by auto => />.
+inline *; auto => />. admit.
+qed.
+
+equiv dec_same :  M.indcpa_dec_jazz ~ Mderand.indcpa_dec_jazz :
+  ={arg,Glob.mem} ==> ={res,Glob.mem}.
+proc.
+inline Mderand.indcpa_dec_compute.
+swap {2} 8 2.
+swap {2} 1 8.
+swap {2} 4 4.
+seq 7 7 : (={Glob.mem,msgp,skp,bp,v}).
+inline *; auto => />; admit. 
+by sim.
+qed.
